int induction

c/poc/strlen_spec.v
@@ -7,7 +7,24 @@ From compcert Require Import Coqlib Integers Floats AST Ctypes Cop Clight Clight
 (* Specification of the strlen function *)
 
 
+Proposition int_ptrofs_mod_eq : (Int.modulus <= Ptrofs.modulus).
+Proof.
+  cbv. destruct Archi.ptr64; congruence.
+Qed.
+
+Proposition ptrofs_mod_1_0 : 0 <= 1 < Ptrofs.modulus.
+Proof.
+  cbv. destruct Archi.ptr64; split; congruence.
+Qed.
+
 Definition int_of_nat :=  fun n => Int.repr (Z.of_nat n).
+
+(* automatically generated induction principle *)
+Hypothesis int_ind : forall P : int -> Prop,
+       (forall (intval : Z) (intrange : -1 < intval < Int.modulus),
+        P {| Int.intval := intval; Int.intrange := intrange |}) ->
+       forall m : int, P m.
+                            
 Inductive strlen_mem (m : mem) (b : block) (ofs : ptrofs) : Z -> Prop :=
 | LengthZeroMem: Mem.loadv Mint8unsigned m (Vptr b ofs) = Some (Vint Int.zero) ->   
                  strlen_mem m b ofs 0
@@ -36,10 +53,10 @@ Inductive strlen_mem_int (m : mem) (b : block) (ofs : ptrofs) : int -> Prop :=
 | LengthZeroMem_int: Mem.loadv Mint8unsigned m (Vptr b ofs) = Some (Vint Int.zero) ->   
                  strlen_mem_int m b ofs Int.zero
 | LengthSuccMem_int: forall n c,
-    strlen_mem_int m b (Ptrofs.add ofs Ptrofs.one) n ->
+    strlen_mem_int m b (Ptrofs.add ofs Ptrofs.one) (Int.repr n) ->
     Mem.loadv Mint8unsigned m (Vptr b ofs)  = Some (Vint c) ->
     c <> Int.zero ->
-    strlen_mem_int m b ofs (Int_succ n).
+    strlen_mem_int m b ofs (Int.repr (Z.succ n)).
 
 
 (* strlen C light AST *)
@@ -263,10 +280,7 @@ Qed.
 
 
  (* add more lemmas from Compcert to ptrofs hints *)
-Proposition int_ptrofs_mod_eq : (Int.modulus <= Ptrofs.modulus).
-Proof.
-  cbv. destruct Archi.ptr64; congruence.
-  Qed.
+
 
 Hint Resolve Ptrofs.mul_one Ptrofs.add_zero int_ptrofs_mod_eq : ptrofs.
 Lemma strlen_to_mem_n : forall len m b ofs, strlen_mem_n m b ofs len ->
@@ -339,64 +353,144 @@ Admitted.
 
 
 Lemma strlen_to_mem_int : forall len m b ofs, strlen_mem_int m b ofs len ->
-                                         forall i, Int.lt i len = true -> exists c, Mem.loadv chunk m (Vptr b (Ptrofs.add ofs (Ptrofs.of_int i))) = Some (Vint c) /\ c <> Int.zero.
+                                         forall i, Int.ltu i len = true -> exists c, Mem.loadv chunk m (Vptr b (Ptrofs.add ofs (Ptrofs.of_int i))) = Some (Vint c) /\ c <> Int.zero.
 Proof.
-  intro len. 
-    eapply (natlike_ind  (fun intval =>  intval = Int.intval len -> forall (m : mem) (b : block) (ofs : ptrofs),
-  strlen_mem_int m b ofs len ->
+  induction len using int_ind.
+  generalize intrange.
+  eapply (natlike_ind (fun intval0 => forall (intrange0 : -1 < intval0 < Int.modulus) 
+    (m : mem) (b : block) (ofs : ptrofs),
+  strlen_mem_int m b ofs
+    {| Int.intval := intval0; Int.intrange := intrange0 |} ->
   forall i : int,
-  Int.lt i len = true ->
+  Int.ltu i
+    {| Int.intval := intval0; Int.intrange := intrange0 |} =
+  true ->
   exists c : int,
-    Mem.loadv chunk m (Vptr b (Ptrofs.add ofs (Ptrofs.of_int i))) = Some (Vint c) /\
-    c <> Int.zero)). 
-    (* Base len *)
-    intro.
-    - assert (len = Int.zero) by admit.
-     rewrite H0.
-     intros.
-     admit. (* contradiction *)
-    (* I.S. len *)
-    - intros until ofs. intro Spec.
-
-    (*  eapply (natlike_ind  (fun intval => forall i, intval = Int.intval i -> 
-          Int.lt i len = true ->
+    Mem.loadv chunk m
+      (Vptr b (Ptrofs.add ofs (Ptrofs.of_int i))) =
+    Some (Vint c) /\ c <> Int.zero)).
+    
+    
+  - (* Base len *)
+    intros.
+    unfold Int.ltu in H0.
+    unfold Int.unsigned in H0.
+    simpl in H0.
+    destruct (zlt (Int.intval i) 0).
+    pose (Int.intrange i).
+    nia.
+    intuition.
+    
+  - (* I.S. len *)
+    intros until ofs. intro Spec.
+    induction i using int_ind.
+    generalize intrange1.
+    eapply (natlike_ind (fun intval0 =>
+                           forall intrange2 : -1 < intval0 < Int.modulus,
+  Int.ltu
+    {| Int.intval := intval0; Int.intrange := intrange2 |}
+    {| Int.intval := Z.succ x; Int.intrange := intrange0 |} =
+  true ->
   exists c : int,
-    Mem.loadv chunk m (Vptr b (Ptrofs.add ofs (Ptrofs.of_int i))) = Some (Vint c) /\
-    c <> Int.zero) ).
+    Mem.loadv chunk m
+      (Vptr b
+         (Ptrofs.add ofs
+            (Ptrofs.of_int
+               {|
+               Int.intval := intval0;
+               Int.intrange := intrange2 |}))) = 
+    Some (Vint c) /\ c <> Int.zero)).
+   
       + (* Base i *)
         intros.
-        assert (i = Int.zero) by admit.
-        rewrite H4.
+        
         inversion Spec.
-        admit. (* contradiction *)
-        rewrite <- H8 in Spec.
-        admit. (* same as in the case of Z *)
+        replace (match Int.zero with
+       | {| Int.intval := intval |} => intval
+                 end) with 0 in H2.
+        nia.
+        { unfold Int.zero.
+          unfold Int.intval.
+          replace 0 with (Int.unsigned (Int.repr 0)) by (auto with ints). auto with ints. }
+          
+          
+      
+       replace (Ptrofs.add ofs
+            (Ptrofs.of_int
+               {|
+               Int.intval := 0;
+               Int.intrange := intrange2 |})) with ofs by (auto with ptrofs).
+       exists c. apply (conj H4 H5).
+
       + (* Ind. step  i*)
-         intros. 
-         assert (x0 < x) by nia.
+      intros. 
       rename H0 into IHlen.
+      assert (intrange_x : -1 < x < Int.modulus) by nia.
+      assert (intrange_x0 : -1 < x0 < Int.modulus) by nia.
+      assert (Int.ltu
+         {|
+         Int.intval := x0;
+         Int.intrange := intrange_x0|}
+         {|
+         Int.intval := x;
+         Int.intrange := intrange_x |} = true) by admit.
       inversion Spec.
-      nia.
-      assert (n = x) by nia.
-      rewrite H8 in H5.
-      pose (IHlen m b (Ptrofs.add ofs Ptrofs.one) H5 x0 H1 H4).
-       replace  (Ptrofs.add ofs (Ptrofs.repr (Z.succ x0))) with (Ptrofs.add (Ptrofs.add ofs Ptrofs.one) (Ptrofs.repr x0)).
+  replace (match Int.zero with
+       | {| Int.intval := intval |} => intval
+       end) with 0 in H4.
+  nia.
+  { unfold Int.zero.
+          unfold Int.intval.
+          replace 0 with (Int.unsigned (Int.repr 0)) by (auto with ints). auto with ints. }
+  replace (match Int.repr (Z.succ n) with
+       | {| Int.intval := intval |} => intval
+       end) with (Z.succ n) in H4.
+  assert (n = x) by nia.
+  rewrite H8 in H5.
+  assert (Int.repr x = {| Int.intval := x; Int.intrange := intrange_x |}) by admit. rewrite H9 in H5. 
+      pose (IHlen intrange_x m b (Ptrofs.add ofs Ptrofs.one) H5 {| Int.intval := x0; Int.intrange := intrange_x0 |} H0).
+       replace 
+       (Ptrofs.add ofs
+            (Ptrofs.of_int
+               {|
+               Int.intval := Z.succ x0;
+               Int.intrange := intrange2 |})) with  (Ptrofs.add (Ptrofs.add ofs Ptrofs.one)
+               (Ptrofs.of_int
+                  {|
+                  Int.intval := x0;
+                  Int.intrange := intrange_x0 |})).
        assumption.
+
+       
        { 
     
-     (*  replace  (Z.succ (Z.of_nat i)) with ((Z.of_nat i) + 1) by (auto with zarith). *)
       rewrite Ptrofs.add_assoc.
       f_equal.
       unfold Ptrofs.add.
+      unfold Ptrofs.of_int.
       f_equal.
       unfold Ptrofs.one.
       repeat rewrite Ptrofs.unsigned_repr_eq.
       repeat rewrite Zmod_small.
+      unfold Int.unsigned.
+      unfold Int.intval.
       nia.
-      admit. (* intrange *)
-      admit.
-             }
-        *)
+      unfold Int.unsigned.
+      unfold Int.intval.
+      pose (int_ptrofs_mod_eq).
+      nia.
+      apply ptrofs_mod_1_0.
+       }
+       {
+         
+      
+    admit.
+
+  }
+      + nia.
+  - nia.
+  
+
 Admitted.
 
 (* Correctness statements *)
